Use list in trees, nat list as paths

Incredible_Completeness.thy
@@ -2,6 +2,9 @@ theory Incredible_Completeness
 imports Natural_Deduction Incredible_Deduction Incredible_Trees
 begin
 
+type_synonym 'form vertex = "('form \<times> nat list)"
+type_synonym ('form, 'var) edge'' = "('form vertex, 'form, 'var) edge'"
+
 locale Solved_Task =
   Abstract_Task  freshenLC renameLCs lconsts closed subst subst_lconsts subst_renameLCs anyP antecedent consequent rules assumptions conclusions
    for freshenLC :: "nat \<Rightarrow> 'var \<Rightarrow> 'var" 
@@ -46,15 +49,15 @@ lemma iwf_pre_it:
   shows "local_iwf (pre_it c) (fst (root (ts c)))"
   using assms by (auto intro!: iwf_to_it ts_finite ts_wf)
 
-definition vertices :: "('form, 'var) vertex fset"  where
-  "vertices = Abs_fset (Union ( set (map (\<lambda> c. insert (c, []) ((\<lambda> p. (c, plain_ant c # p)) ` (it_paths (pre_it c))))  conclusions)))"
+definition vertices :: "'form vertex fset"  where
+  "vertices = Abs_fset (Union ( set (map (\<lambda> c. insert (c, []) ((\<lambda> p. (c, 0 # p)) ` (it_paths (pre_it c))))  conclusions)))"
 
 text {* For the remaining time, work with the tree with global freshness. *}
 
 abbreviation it' where
   "it' c \<equiv> globalize (to_it (ts c))"
 
-lemma mem_vertices: "v |\<in>| vertices \<longleftrightarrow>  (fst v \<in> set conclusions \<and> (snd v = [] \<or> snd v \<in> (op # (plain_ant (fst v))) ` it_paths (it' (fst v))))"
+lemma mem_vertices: "v |\<in>| vertices \<longleftrightarrow>  (fst v \<in> set conclusions \<and> (snd v = [] \<or> snd v \<in> (op # 0) ` it_paths (it' (fst v))))"
   unfolding vertices_def fmember.rep_eq ffUnion.rep_eq 
   by (cases v)(auto simp add: Abs_fset_inverse Bex_def it_paths_globalize)
 
@@ -64,19 +67,19 @@ lemma prefixeq_vertices: "(c,is) |\<in>| vertices \<Longrightarrow> prefixeq is'
 lemma none_vertices[simp]: "(c, []) |\<in>| vertices \<longleftrightarrow> c \<in> set conclusions"
   by (simp add: mem_vertices)
 
-lemma some_vertices[simp]: "(c, i#is) |\<in>| vertices \<longleftrightarrow> c \<in> set conclusions \<and> i = plain_ant c \<and> is \<in> it_paths (it' c)"
+lemma some_vertices[simp]: "(c, i#is) |\<in>| vertices \<longleftrightarrow> c \<in> set conclusions \<and> i = 0 \<and> is \<in> it_paths (it' c)"
   by (auto simp add: mem_vertices)
 
 lemma vertices_cases[consumes 1, case_names None Some]:
   assumes "v |\<in>| vertices"
   obtains c where "c \<in> set conclusions" and "v = (c, [])"
-      |   c "is" where "c \<in> set conclusions" and "is \<in> it_paths (it' c)" and "v = (c, plain_ant c#is)"
+      |   c "is" where "c \<in> set conclusions" and "is \<in> it_paths (it' c)" and "v = (c, 0#is)"
 using assms by (cases v; rename_tac "is"; case_tac "is"; auto)
 
 lemma vertices_induct[consumes 1, case_names None Some]:
   assumes "v |\<in>| vertices"
   assumes "\<And> c. c \<in> set conclusions \<Longrightarrow> P (c, [])"
-  assumes "\<And> c is . c \<in> set conclusions \<Longrightarrow> is \<in> it_paths (it' c) \<Longrightarrow> P (c, plain_ant c#is)"
+  assumes "\<And> c is . c \<in> set conclusions \<Longrightarrow> is \<in> it_paths (it' c) \<Longrightarrow> P (c, 0#is)"
   shows "P v"
 using assms by (cases v; rename_tac "is"; case_tac "is"; auto)
 
@@ -87,7 +90,7 @@ lemma global_iwf_it:
 
 text {* Start building the graph *}
 
-fun nodeOf :: "('form, 'var) vertex \<Rightarrow> ('form, 'rule) graph_node" where
+fun nodeOf :: "'form vertex \<Rightarrow> ('form, 'rule) graph_node" where
   "nodeOf (pf, []) = Conclusion pf"
 | "nodeOf (pf, i#is) = iNodeOf (tree_at (it' pf) is)"
 
@@ -108,28 +111,32 @@ lemma terminal_is_nil[simp]: "v |\<in>| vertices \<Longrightarrow> outPorts (nod
 sublocale Vertex_Graph nodes inPorts outPorts vertices nodeOf.
 
 
-definition edge_from :: "'form \<Rightarrow> ('form, 'var) in_port list => (('form, 'var) vertex \<times> ('form,'var) out_port)" where 
-  "edge_from c is = ((c, plain_ant c # is),  Reg (iOutPort (tree_at (it' c) is)))"
+definition edge_from :: "'form \<Rightarrow> nat list => ('form vertex \<times> ('form,'var) out_port)" where 
+  "edge_from c is = ((c, 0 # is),  Reg (iOutPort (tree_at (it' c) is)))"
 
-lemma fst_edge_from[simp]: "fst (edge_from c is) = (c, plain_ant c # is)"
+lemma fst_edge_from[simp]: "fst (edge_from c is) = (c, 0 # is)"
   by (simp add: edge_from_def)
 
-definition edge_to :: "'form \<Rightarrow> ('form, 'var) in_port list => (('form, 'var) vertex \<times> ('form,'var) in_port)"  where
+fun in_port_at :: "('form \<times> nat list) \<Rightarrow> nat \<Rightarrow> ('form,'var) in_port" where
+    "in_port_at (c, [])  _  = plain_ant c"
+  | "in_port_at (c, _#is) i = inPorts' (iNodeOf (tree_at (it' c) is)) ! i"
+
+definition edge_to :: "'form \<Rightarrow> nat list => ('form vertex \<times> ('form,'var) in_port)"  where
  "edge_to c is =
-    (case rev is of   []   \<Rightarrow> ((c, []),            plain_ant c)
-                    | i#is \<Rightarrow> ((c, plain_ant c # (rev is)), i))"
+    (case rev is of   []   \<Rightarrow> ((c, []),           in_port_at (c, []) 0)
+                    | i#is \<Rightarrow> ((c, 0 # (rev is)), in_port_at (c, (0#rev is)) i))"
 
 lemma edge_to_Nil[simp]: "edge_to c [] = ((c, []), plain_ant c)"
   by (simp add: edge_to_def)
 
-lemma edge_to_Snoc[simp]: "edge_to c (is@[i]) = ((c, plain_ant c # is), i)"
+lemma edge_to_Snoc[simp]: "edge_to c (is@[i]) = ((c, 0 # is), in_port_at ((c, 0 # is)) i)"
   by (simp add: edge_to_def)
 
-definition edge_at :: "'form \<Rightarrow> ('form, 'var) in_port list => ('form, 'var) edge''"  where
-   "edge_at c i = (edge_from c i, edge_to c i)"
+definition edge_at :: "'form \<Rightarrow> nat list => ('form, 'var) edge''"  where
+   "edge_at c is = (edge_from c is, edge_to c is)"
 
-lemma fst_edge_at[simp]: "fst (edge_at c i) = edge_from c i" by (simp add: edge_at_def)
-lemma snd_edge_at[simp]: "snd (edge_at c i) = edge_to c i" by (simp add: edge_at_def)
+lemma fst_edge_at[simp]: "fst (edge_at c is) = edge_from c is" by (simp add: edge_at_def)
+lemma snd_edge_at[simp]: "snd (edge_at c is) = edge_to c is" by (simp add: edge_at_def)
 
 
 lemma pre_hyps_exist:
@@ -168,14 +175,16 @@ qed
 
 
 
-definition hyp_edge_to where
-  "hyp_edge_to c is = ((c, plain_ant c # is),  plain_ant anyP)"
+definition hyp_edge_to :: "'form \<Rightarrow> nat list => ('form vertex \<times> ('form,'var) in_port)" where
+  "hyp_edge_to c is = ((c, 0 # is),  plain_ant anyP)"
 
-definition hyp_edge_from where
+(* TODO: Replace n and s by "subst s (freshen n anyP)" *)
+definition hyp_edge_from :: "'form \<Rightarrow> nat list => nat \<Rightarrow> 'subst \<Rightarrow> ('form vertex \<times> ('form,'var) out_port)" where
   "hyp_edge_from c is n s = 
-    ((c, plain_ant c # hyp_port_path_for (it' c) is (subst s (freshen n anyP))), hyp_port_h_for (it' c) is (subst s (freshen n anyP)))"
+    ((c, 0 # hyp_port_path_for (it' c) is (subst s (freshen n anyP))),
+     hyp_port_h_for (it' c) is (subst s (freshen n anyP)))"
 
-definition hyp_edge_at where
+definition hyp_edge_at  :: "'form \<Rightarrow> nat list => nat \<Rightarrow> 'subst \<Rightarrow> ('form, 'var) edge''" where
   "hyp_edge_at c is n s = (hyp_edge_from c is n s, hyp_edge_to c is)"
 
 lemma fst_hyp_edge_at[simp]:
@@ -200,8 +209,12 @@ lemma edge_to_valid_in_port:
   assumes "p \<in> it_paths (it' c)"
   assumes "c \<in> set conclusions"
   shows "valid_in_port (edge_to c p)"
-using assms
-by (auto simp add: edge_to_def split: list.split elim!: it_path_SnocE)
+  using assms
+  apply (auto simp add: edge_to_def inPorts_fset_of split: list.split elim!: it_paths_SnocE)
+  apply (rule nth_mem)
+  apply (drule (1) iwf_length_inPorts[OF global_iwf_it])
+  apply auto
+  done
 
 lemma hyp_edge_from_valid_out_port:
   assumes "is \<in> it_paths (it' c)"
@@ -220,11 +233,12 @@ using assms by (auto simp add: hyp_edge_to_def)
 
 
 
-inductive scope' where
+inductive scope' :: "'form vertex \<Rightarrow> ('form,'var) in_port \<Rightarrow> 'form \<times> nat list \<Rightarrow> bool" where
   "c \<in> set conclusions \<Longrightarrow>
-   is' \<in> (op # (plain_ant c)) ` it_paths (it' c) \<Longrightarrow>
+   is' \<in> (op # 0) ` it_paths (it' c) \<Longrightarrow>
    prefixeq (is@[i]) is' \<Longrightarrow> 
-   scope' (c, is) i (c, is')"
+   ip = in_port_at (c,is) i \<Longrightarrow>
+   scope' (c, is) ip (c, is')"
 
 inductive_simps scope_simp: "scope' v i v'"
 inductive_cases scope_cases: "scope' v i v'"
@@ -234,8 +248,9 @@ lemma scope_valid:
 by (auto elim: scope_cases)
 
 lemma scope_valid_inport:
-  "valid_in_port (v, i) \<Longrightarrow> v' |\<in>| vertices \<Longrightarrow> scope' v i v' \<longleftrightarrow> fst v = fst v' \<and> prefixeq (snd v@[i]) (snd v')"
-by (cases v; cases v') (auto simp add: scope'.simps mem_vertices)
+  "v' |\<in>| vertices \<Longrightarrow> scope' v ip  v' \<longleftrightarrow> (\<exists> i. fst v = fst v' \<and> prefixeq (snd v@[i]) (snd v') \<and> ip = in_port_at v i)"
+by (cases v; cases v')  (auto simp add: scope'.simps mem_vertices)
+
 
 fun inits where
   "inits [] = [[]]"
@@ -252,7 +267,7 @@ by (cases "is" rule: rev_cases) auto
 lemma in_set_inits[simp]: "is' \<in> set (inits is) \<longleftrightarrow> prefixeq is' is"
   by (induction "is'" arbitrary: "is"; case_tac "is"; auto)
 
-definition terminal_path_from :: "'form \<Rightarrow> ('form, 'var) in_port list => ('form, 'var) edge'' list" where
+definition terminal_path_from :: "'form \<Rightarrow> nat list => ('form, 'var) edge'' list" where
    "terminal_path_from c is = map (edge_at c) (rev (inits is))"
 
 lemma terminal_path_from_Nil[simp]:
@@ -260,30 +275,32 @@ lemma terminal_path_from_Nil[simp]:
   by (simp add: terminal_path_from_def)
 
 lemma terminal_path_from_Snoc[simp]:
-  "terminal_path_from c (is @ [i]) = edge_at c (is@[i]) # terminal_path_from c is"
+  "terminal_path_from c (is @ [i]) = edge_at  c (is@[i]) # terminal_path_from c is"
   by (simp add: terminal_path_from_def)
 
 lemma path_terminal_path_from:
   "c \<in> set conclusions \<Longrightarrow>
   is \<in> it_paths (it' c) \<Longrightarrow>
-  path (c, plain_ant c # is) (c, []) (terminal_path_from c is)"
+  path (c, 0 # is) (c, []) (terminal_path_from c is)"
 by (induction "is" rule: rev_induct)
-   (auto simp add: path_cons_simp intro!: regular_edge elim: it_path_SnocE)
+   (auto simp add: path_cons_simp intro!: regular_edge elim: it_paths_SnocE)
 
 lemma edge_step:
   assumes "(((a, b), ba), ((aa, bb), bc)) \<in> edges"
-  obtains "a = aa" and "b = bb@[bc]" and "hyps (nodeOf (a, b)) ba = None"
-  | i where "a = aa" and "prefixeq (b@[i]) bb" and "hyps (nodeOf (a, b)) ba = Some i"
+  obtains 
+    i where "a = aa" and "b = bb@[i]" and "bc = in_port_at (aa,bb) i"  and "hyps (nodeOf (a, b)) ba = None"
+  | i where "a = aa" and "prefixeq (b@[i]) bb" and "hyps (nodeOf (a, b)) ba = Some (in_port_at (a,b) i)"
 using assms
 proof(cases rule: edges.cases[consumes 1, case_names Reg Hyp])
   case (Reg c "is")
-  hence "a = aa" and "b = bb@[bc]" and "hyps (nodeOf (a, b)) ba = None"
+  then obtain i where  "a = aa" and "b = bb@[i]" and "bc = in_port_at (aa,bb) i"  and "hyps (nodeOf (a, b)) ba = None"
     by (auto elim!: edges.cases simp add: edge_at_def edge_from_def edge_to_def split: list.split list.split_asm)
   thus thesis by (rule that)
 next
   case (Hyp c "is" n s)
-  hence "a = aa" and "prefixeq (b@[hyp_port_i_for (it' c) is (subst s (freshen n anyP))]) bb" and
-    "hyps (nodeOf (a, b)) ba = Some (hyp_port_i_for (it' c) is (subst s (freshen n anyP)))"
+  let ?i = "hyp_port_i_for (it' c) is (subst s (freshen n anyP))"
+  from Hyp have "a = aa" and "prefixeq (b@[?i]) bb" and
+    "hyps (nodeOf (a, b)) ba = Some (in_port_at (a,b) ?i)"
   by (auto simp add: edge_at_def edge_from_def edge_to_def hyp_edge_at_def hyp_edge_to_def hyp_edge_from_def
       intro: hyp_port_prefixeq hyps_exist' hyp_port_hyps)
   thus thesis by (rule that)
@@ -293,11 +310,10 @@ lemma path_has_prefixes:
   assumes "path v v' pth"
   assumes "snd v' = []"
   assumes "prefixeq (is' @ [i]) (snd v)"
-  shows "((fst v, is'), i) \<in> snd ` set pth"
+  shows "((fst v, is'), (in_port_at (fst v, is') i)) \<in> snd ` set pth"
   using assms
   by (induction rule: path.induct)(auto elim!: edge_step dest: prefixeq_snocD)
-
-
+  
 lemma in_scope: "valid_in_port (v', p') \<Longrightarrow> v \<in> scope (v', p') \<longleftrightarrow> scope' v' p' v"
 proof
   assume "v \<in> scope (v', p')"
@@ -314,7 +330,7 @@ proof
     case (Some c "is")
 
     from `c \<in> set conclusions` `is \<in> it_paths (it' c)`
-    have "path (c, plain_ant c # is) (c, []) (terminal_path_from c is)"
+    have "path (c, 0#is) (c, []) (terminal_path_from c is)"
       by (rule path_terminal_path_from)
     moreover
     from `c \<in> set conclusions`
@@ -326,7 +342,7 @@ proof
       unfolding terminal_path_from_def by auto
     then obtain is' where "prefixeq is' is" and "(v',p') = edge_to c is'"
       by auto
-    show "scope' v' p' (c, plain_ant c # is)"
+    show "scope' v' p' (c, 0#is)"
     proof(cases "is'" rule: rev_cases)
       case Nil
       with `(v',p') = edge_to c is'`
@@ -337,7 +353,7 @@ proof
     next
       case (snoc is'' i)
       with `(v',p') = edge_to c is'`
-      have "v' = (c, plain_ant c # is'')" and "p' = i"
+      have "v' = (c, 0 # is'')" and "p' = in_port_at v' i"
         by (auto simp add: edge_to_def)
       with `c \<in> set conclusions` `is \<in> it_paths (it' c)` `prefixeq is' is`[unfolded snoc]
       show ?thesis
@@ -347,9 +363,10 @@ proof
 next
   assume "valid_in_port (v', p')"
   assume "scope' v' p' v"
-  then obtain c is' "is" where
+  then obtain c is' i "is" where
     "v' = (c, is')" and "v = (c, is)" and "c \<in> set conclusions" and
-    "is \<in> op # (plain_ant c) ` it_paths (it' c)" and  "prefixeq (is' @ [p']) is"
+    "p' = in_port_at v' i" and
+    "is \<in> op # 0 ` it_paths (it' c)" and  "prefixeq (is' @ [i]) is"
     by (auto simp add: scope'.simps)
 
   from `scope' v' p' v`
@@ -362,8 +379,8 @@ next
     assume "terminal_vertex t"
     hence "snd t = []" by auto
 
-    from path_has_prefixes[OF `path (c,is) t pth` `snd t = []`, simplified, OF `prefixeq (is' @ [p']) is`]
-    show "((c, is'), p') \<in> snd ` set pth".
+    from path_has_prefixes[OF `path (c,is) t pth` `snd t = []`, simplified, OF `prefixeq (is' @ [i]) is`]
+    show "((c, is'), p') \<in> snd ` set pth" unfolding `p' = _ ` `v' = _ `.
   qed
   thus "v \<in> scope (v', p')" using `v =_` `v' = _` by simp
 qed
@@ -393,8 +410,8 @@ lemma hyps_free_path_length:
   shows "length pth + length (snd v') = length (snd v)"
 using assms by induction (auto elim!: edge_step )
 
-fun vidx :: "('form, 'var) vertex \<Rightarrow> nat" where
-  "vidx (c, []) = fidx conc_forms c"
+fun vidx :: "'form vertex \<Rightarrow> nat" where
+  "vidx (c, [])   = fidx conc_forms c"
  |"vidx (c, _#is) = iAnnot (tree_at (it' c) is)"
 
 lemma vidx_inj: "inj_on vidx (fset vertices)"
@@ -406,8 +423,7 @@ proof
   show "inj_on vidx (fset vertices)" by (rule vidx_inj)
 qed
 
-sublocale Tasked_Proof_Graph freshenLC renameLCs lconsts closed subst subst_lconsts subst_renameLCs anyP antecedent consequent fresh_vars rules assumptions conclusions
-  vertices nodeOf edges vidx inst
+sublocale  Well_Scoped_Graph nodes inPorts outPorts vertices nodeOf edges hyps
 proof
   fix v\<^sub>1 p\<^sub>1 v\<^sub>2 p\<^sub>2 p'
   assume assms: "((v\<^sub>1, p\<^sub>1), (v\<^sub>2, p\<^sub>2)) \<in> edges" "hyps (nodeOf v\<^sub>1) p\<^sub>1 = Some p'"
@@ -416,21 +432,25 @@ proof
     using valid_edges by auto
 
   from assms
-  have "fst v\<^sub>1 = fst v\<^sub>2 \<and> prefixeq (snd v\<^sub>1@[p']) (snd v\<^sub>2)"
+  have "\<exists> i. fst v\<^sub>1 = fst v\<^sub>2 \<and> prefixeq (snd v\<^sub>1@[i]) (snd v\<^sub>2) \<and> p' = in_port_at v\<^sub>1 i"
     by (cases v\<^sub>1; cases v\<^sub>2; auto elim!: edge_step)
   hence "scope' v\<^sub>1 p' v\<^sub>2"
-    unfolding scope_valid_inport[OF `valid_in_port (v\<^sub>1, p')` `v\<^sub>2 |\<in>| vertices`].
+    unfolding scope_valid_inport[OF `v\<^sub>2 |\<in>| vertices`].
   hence "v\<^sub>2 \<in> scope (v\<^sub>1, p')"
     unfolding in_scope[OF `valid_in_port (v\<^sub>1, p')`].
   thus "(v\<^sub>2, p\<^sub>2) = (v\<^sub>1, p') \<or> v\<^sub>2 \<in> scope (v\<^sub>1, p')" ..
-  next
+qed
 
+sublocale Acyclic_Graph nodes inPorts outPorts vertices nodeOf edges hyps 
+proof
   fix v pth
   assume "path v v pth" and "hyps_free pth"
   from hyps_free_path_length[OF this]
   show "pth = []" by simp
-  next
+qed
 
+sublocale Saturated_Graph nodes inPorts outPorts vertices nodeOf edges
+proof
   fix v p
   assume "valid_in_port (v, p)"
   thus "\<exists>e\<in>edges. snd e = (v, p)"
@@ -456,21 +476,30 @@ proof
     next
       case (Cons c' "is")
       with `valid_in_port ((c, cis), p)`
-      have [simp]: "c' = plain_ant c" and "is \<in> it_paths (it' c)"
+      have [simp]: "c' = 0" and "is \<in> it_paths (it' c)"
         and "p |\<in>| inPorts (iNodeOf (tree_at (it' c) is))" by auto
+       
+      from this(3) obtain i where
+        "i < length (inPorts' (iNodeOf (tree_at (it' c) is)))" and
+        "p = inPorts' (iNodeOf (tree_at (it' c) is)) ! i"
+          by (auto simp add: inPorts_fset_of in_set_conv_nth)
+
       show ?thesis
       proof (cases "tree_at (it' c) is")
         case INode
         hence "\<not> isHNode (tree_at (it' c) is)" by simp
-        from global_iwf_it[OF `c \<in> set conclusions`] `is \<in> it_paths (it' c)` this `p |\<in>| inPorts (iNodeOf (tree_at (it' c) is))`
-        have "is@[p] \<in> it_paths (it' c)" by (rule it_path_SnocI)
+        from iwf_length_inPorts_not_HNode[OF global_iwf_it[OF `c \<in> set conclusions`]  `is \<in> it_paths (it' c)` this]
+             `i < length (inPorts' (iNodeOf (tree_at (it' c) is)))`
+        have "i < length (iAnts (tree_at (it' c) is))" by simp
+        with `is \<in> it_paths (it' c)`
+        have "is@[i] \<in> it_paths (it' c)" by (rule it_path_SnocI)
         from `c \<in> set conclusions` this
-        have "edge_at c (is@[p]) \<in> edges" by (rule regular_edge)
+        have "edge_at c (is@[i]) \<in> edges" by (rule regular_edge)
         moreover
-        have "snd (edge_at c (is@[p])) = ((c, plain_ant c # is), p)"
+        have "snd (edge_at c (is@[i])) = ((c, 0 # is),  inPorts' (iNodeOf (tree_at (it' c) is)) ! i)"
           by (simp add: edge_to_def)
         ultimately
-        show ?thesis by (auto simp add: Cons simp del: snd_edge_at)
+        show ?thesis by (auto simp add: Cons `p = _` simp del: snd_edge_at)
       next
         case (HNode n s)
         from `c \<in> set conclusions` `is \<in> it_paths (it' c)`  this
@@ -479,15 +508,17 @@ proof
         from HNode `p |\<in>| inPorts (iNodeOf (tree_at (it' c) is))`
         have [simp]: "p = plain_ant anyP" by simp
 
-        have "snd (hyp_edge_at c is n s) = ((c, plain_ant c # is), p)"
+        have "snd (hyp_edge_at c is n s) = ((c, 0 # is), p)"
           by (simp add: hyp_edge_to_def)
         ultimately
         show ?thesis by (auto simp add: Cons simp del: snd_hyp_edge_at)
       qed
     qed
    qed
-  next
-  
+qed
+
+sublocale Pruned_Port_Graph nodes inPorts outPorts vertices nodeOf edges
+proof
   fix v 
   assume "v |\<in>| vertices"
   thus "\<exists>pth v'. path v v' pth \<and> terminal_vertex v'"
@@ -498,15 +529,19 @@ proof
     show ?case by blast
   next
     case (Some c "is")
-    hence "path (c, plain_ant c # is) (c, []) (terminal_path_from c is)"
+    hence "path (c, 0 # is) (c, []) (terminal_path_from c is)"
       by (rule path_terminal_path_from)
     moreover
     have "terminal_vertex (c,[])" using Some(1) by simp
     ultimately
     show ?case by blast
   qed
-  next
+qed
 
+sublocale Well_Shaped_Graph  nodes inPorts outPorts vertices nodeOf edges hyps..
+
+sublocale Solution inPorts outPorts nodeOf hyps nodes vertices  labelsIn labelsOut freshenLC renameLCs lconsts closed subst subst_lconsts subst_renameLCs anyP vidx inst edges
+proof
   fix v\<^sub>1 p\<^sub>1 v\<^sub>2 p\<^sub>2
   assume "((v\<^sub>1, p\<^sub>1), (v\<^sub>2, p\<^sub>2)) \<in> edges"
   thus "labelAtOut v\<^sub>1 p\<^sub>1 = labelAtIn v\<^sub>2 p\<^sub>2"
@@ -515,7 +550,7 @@ proof
    
     from `((v\<^sub>1, p\<^sub>1), v\<^sub>2, p\<^sub>2) = edge_at c is`
     have "(v\<^sub>1,p\<^sub>1) = edge_from c is" using fst_edge_at by (metis fst_conv)
-    hence [simp]: "v\<^sub>1 = (c, plain_ant c # is)" by (simp add: edge_from_def)
+    hence [simp]: "v\<^sub>1 = (c, 0 # is)" by (simp add: edge_from_def)
 
     show ?thesis
     proof(cases "is" rule:rev_cases)
@@ -537,10 +572,11 @@ proof
       have "labelAtOut v\<^sub>1 p\<^sub>1 = subst (iSubst ?t1) (freshen (vidx v\<^sub>1) (iOutPort ?t1))"
         using regular_edge snoc by (simp add: labelAtOut_def edge_at_def edge_from_def)
       also have "vidx v\<^sub>1 = iAnnot ?t1" using snoc regular_edge(3) by simp
-      also have "subst (iSubst ?t1) (freshen (iAnnot ?t1) (iOutPort ?t1)) = subst (iSubst ?t2) (freshen (iAnnot ?t2) (a_conc i))"
+      also have "subst (iSubst ?t1) (freshen (iAnnot ?t1) (iOutPort ?t1))
+          = subst (iSubst ?t2) (freshen (iAnnot ?t2) (a_conc (inPorts' (iNodeOf ?t2) ! i)))"
         by (rule iwf_edge_match[OF global_iwf_it[OF `c \<in> set conclusions`] `is \<in> it_paths (it' c)`[unfolded snoc]])
-      also have "iAnnot ?t2 = vidx (c, plain_ant c # is')" by simp
-      also have "subst (iSubst ?t2) (freshen (vidx (c, plain_ant c # is')) (a_conc i)) = labelAtIn v\<^sub>2 p\<^sub>2"
+      also have "iAnnot ?t2 = vidx (c, 0 # is')" by simp
+      also have "subst (iSubst ?t2) (freshen (vidx (c, 0 # is')) (a_conc (inPorts' (iNodeOf ?t2) ! i))) = labelAtIn v\<^sub>2 p\<^sub>2"
         using regular_edge snoc by (simp add: labelAtIn_def edge_at_def)
       finally show ?thesis.
   qed
@@ -558,7 +594,7 @@ proof
 
     from `((v\<^sub>1, p\<^sub>1), v\<^sub>2, p\<^sub>2) = hyp_edge_at c is n s`
     have "(v\<^sub>1,p\<^sub>1) = hyp_edge_from c is n s" using fst_hyp_edge_at by (metis fst_conv)
-    hence [simp]: "v\<^sub>1 = (c, plain_ant c # ?his)" by (simp add: hyp_edge_from_def)
+    hence [simp]: "v\<^sub>1 = (c, 0 # ?his)" by (simp add: hyp_edge_from_def)
 
 
     have "labelAtOut v\<^sub>1 p\<^sub>1 = subst (iSubst ?t1) (freshen (vidx v\<^sub>1) (labelsOut (iNodeOf ?t1) ?h))"
@@ -570,15 +606,23 @@ proof
         using hyp_edge by (simp add: labelAtIn_def  hyp_edge_at_def hyp_edge_to_def)
     finally show ?thesis.
   qed
-  next
+qed
 
+sublocale Well_Scoped_Instantiation  freshenLC renameLCs lconsts closed subst subst_lconsts subst_renameLCs anyP inPorts outPorts nodeOf hyps  nodes vertices labelsIn labelsOut vidx inst edges local_vars
+proof
   fix v p var v'
   assume "valid_in_port (v, p)"
   then obtain c "is" where "v = (c,is)" by (cases v, auto)
 
   from `valid_in_port (v, p)` `v= _`
-  have "(c,is) |\<in>| vertices" by simp
+  have "(c,is) |\<in>| vertices"  and "p |\<in>| inPorts (nodeOf (c, is))" by simp_all
   hence "c \<in> set conclusions" by (simp add: mem_vertices)
+
+  from `p |\<in>| _` obtain i where
+    "i < length (inPorts' (nodeOf (c, is)))" and
+    "p = inPorts' (nodeOf (c, is)) ! i" by (auto simp add: inPorts_fset_of in_set_conv_nth)
+  hence "p = in_port_at (c, is) i" by (cases "is") auto
+
 
   assume "var \<in> local_vars (nodeOf v) p"
   hence "var \<in> a_fresh p" by simp
@@ -600,21 +644,25 @@ proof
   from `(c',is'') |\<in>| vertices` `(c,is) |\<in>| vertices` `vidx (c,is) = vidx (c', is'')`
   have "c' = c" and "is'' = is"  by (auto dest: Fun.inj_onD[OF vidx_inj] simp add: fmember.rep_eq)
 
-  have "prefixeq (is @ [p]) is'" sorry
+  have "prefixeq (is @ [i]) is'" sorry
 
   have "is' \<noteq> []" sorry
   with `v' |\<in>| vertices` `v' = _`
   obtain is'' where
-    "is' = plain_ant c' # is''"  and "is'' \<in> it_paths (it' c')"
+    "is' = 0 # is''"  and "is'' \<in> it_paths (it' c')"
       by (auto elim: vertices_cases)
-
-  from `c \<in> set conclusions`  `is'' \<in> it_paths (it' c')` `prefixeq (is @ [p]) is'`
+ 
+  from `c \<in> set conclusions`  `is'' \<in> it_paths (it' c')` `prefixeq (is @ [i]) is'` `p = in_port_at (c, is) i`
   have "scope' v p v'"
-  unfolding `v=_` `v'=_` `c' = _` `is' = _`
-    by (auto intro!: scope'.intros)
+  unfolding `v=_` `v'=_` `c' = _` `is' = _`  by (auto intro: scope'.intros)
   thus "v' \<in> scope (v, p)" using `valid_in_port (v, p)` by (simp add: in_scope)
-  next
+qed
 
+sublocale Scoped_Proof_Graph freshenLC renameLCs lconsts closed subst subst_lconsts subst_renameLCs anyP  inPorts outPorts nodeOf hyps nodes vertices labelsIn labelsOut vidx inst edges local_vars..
+   
+sublocale Tasked_Proof_Graph freshenLC renameLCs lconsts closed subst subst_lconsts subst_renameLCs anyP antecedent consequent fresh_vars rules assumptions conclusions
+  vertices nodeOf edges vidx inst
+proof
   show "set (map Conclusion conclusions) \<subseteq> nodeOf ` fset vertices"
   proof-
   {
@@ -626,8 +674,6 @@ proof
     hence "Conclusion c \<in> nodeOf ` fset vertices"  by simp
   } thus ?thesis by auto
   qed
-  
-qed
-    
+qed  
 
 end
